LeanMove/Tests/Parsing/AllParseTests.lean
@@ -40,6 +40,7 @@ import LeanMove.Tests.Parsing.Test_enum_invalid_ref_unpack_loop
 import LeanMove.Tests.Parsing.Test_enum_borrow_owned
 import LeanMove.Tests.Parsing.Test_comparison_ops
 import LeanMove.Tests.Parsing.Test_casts
+import LeanMove.Tests.Parsing.Test_bitwise
 
 /-! ## All Parse Tests
 
